some failed tests

Impl/CacheImpl.i.dfy
@@ -64,7 +64,8 @@ module CacheImpl {
     predicate Inv()
     {
       && LCMM.Inv(cache)
-      && (forall ref | ref in cache.contents :: cache.contents[ref].Inv())
+      && (forall ref | ref in cache.contents :: 
+        cache.contents[ref].Inv() && BT.WFNode(cache.contents[ref].I()))
     }
 
     // [yizhou7]: free method is tricker than I thought
@@ -162,7 +163,7 @@ module CacheImpl {
 
     linear inout method Insert(ref: BT.G.Reference, linear node: Node)
     requires old_self.Inv()
-    requires node.Inv()
+    requires node.Inv() && BT.WFNode(node.I())
     requires |old_self.I()| <= 0x10000
     ensures self.Inv()
     ensures self.I() == old_self.I()[ref := node.I()]
@@ -177,6 +178,7 @@ module CacheImpl {
         case lNone() => { }
       }
       assert self.cache.contents[ref] == node;
+      // assert BT.WFNode(node.I());
       assert self.Inv();
     }
 
@@ -185,9 +187,10 @@ module CacheImpl {
     requires old_self.Inv()
     requires old_self.ptr(ref).Some?
     requires |old_self.I()| <= 0x10000
-    requires newNode.Inv()
+    requires newNode.Inv() && BT.WFNode(newNode.I())
+
     ensures self.Inv()
-    ensures oldNode.Inv()
+    ensures oldNode.Inv() && BT.WFNode(oldNode.I())
     ensures |self.I()| == |old_self.I()|
     ensures oldNode == old_self.ptr(ref).value
     ensures self.I() == old_self.I()[ref := newNode.I()]
@@ -210,7 +213,8 @@ module CacheImpl {
     requires old_self.Inv()
     requires old_self.ptr(ref).Some?
     ensures self.Inv()
-    ensures node.Inv()
+    ensures node.Inv() && BT.WFNode(node.I())
+
     ensures node == old_self.ptr(ref).value
     ensures self.I() == MapRemove1(old_self.I(), ref)
     {
@@ -243,7 +247,7 @@ module CacheImpl {
     linear inout method MoveAndReplace(oldref: BT.G.Reference,
       newref: BT.G.Reference, linear node: Node)
     requires old_self.Inv()
-    requires node.Inv()
+    requires node.Inv() && BT.WFNode(node.I())
     requires |old_self.I()| <= 0x10000
     requires oldref in old_self.I()
     ensures self.Inv()
@@ -267,7 +271,7 @@ module CacheImpl {
     // Like Insert, but with slightly different requires
     linear inout method Overwrite(ref: BT.G.Reference, linear node: Node)
     requires old_self.Inv()
-    requires node.Inv()
+    requires node.Inv() && BT.WFNode(node.I())
     requires ref in old_self.I()
     requires |old_self.I()| <= 0x10000
     ensures self.Inv()
@@ -298,6 +302,7 @@ module CacheImpl {
       linear var node := inout self.RemoveAndGet(ref);
       inout node.UpdateSlot(slot, bucket, childref);
       newchildren := node.children;
+      assert BT.WFNode(node.I());
       inout self.Insert(ref, node);
     }
 
@@ -308,7 +313,7 @@ module CacheImpl {
     requires BT.WFNode(old_self.I()[ref])
     requires Pivots.BoundedKey(old_self.I()[ref].pivotTable, key)
     requires WeightBucketList(old_self.I()[ref].buckets) + WeightKey(key) 
-      + WeightMessage(msg) < 0x1_0000_0000_0000_0000
+      + WeightMessage(msg) < MaxTotalBucketWeight()
     ensures self.Inv()
     ensures self.I() == old_self.I()
       [ref := BT.NodeInsertKeyValue(old_self.I()[ref], key, msg)]
@@ -318,124 +323,124 @@ module CacheImpl {
       inout self.Insert(ref, node);
     }
 
-    linear inout method SplitParent(ref: BT.G.Reference, slot: uint64, pivot: Key,
-      left_childref: BT.G.Reference, right_childref: BT.G.Reference)
-    requires old_self.Inv()
-    requires old_self.ptr(ref).Some?
-    requires BT.WFNode(old_self.I()[ref])
-    requires old_self.I()[ref].children.Some?
-    requires 0 <= slot as int < |old_self.I()[ref].children.value|
-    requires 0 <= slot as int < |old_self.I()[ref].buckets|
-    requires |old_self.I()| <= 0x10000
-    ensures self.Inv()
-    ensures self.I() == old_self.I()[ref := BT.SplitParent(old_self.I()[ref],
-      pivot, slot as int, left_childref, right_childref)]
-    {
-      linear var node := inout self.RemoveAndGet(ref);
-      inout node.SplitParent(slot, pivot, left_childref, right_childref);
-      inout self.Insert(ref, node);
-    }
+  //   linear inout method SplitParent(ref: BT.G.Reference, slot: uint64, pivot: Key,
+  //     left_childref: BT.G.Reference, right_childref: BT.G.Reference)
+  //   requires old_self.Inv()
+  //   requires old_self.ptr(ref).Some?
+  //   requires BT.WFNode(old_self.I()[ref])
+  //   requires old_self.I()[ref].children.Some?
+  //   requires 0 <= slot as int < |old_self.I()[ref].children.value|
+  //   requires 0 <= slot as int < |old_self.I()[ref].buckets|
+  //   requires |old_self.I()| <= 0x10000
+  //   ensures self.Inv()
+  //   ensures self.I() == old_self.I()[ref := BT.SplitParent(old_self.I()[ref],
+  //     pivot, slot as int, left_childref, right_childref)]
+  //   {
+  //     linear var node := inout self.RemoveAndGet(ref);
+  //     inout node.SplitParent(slot, pivot, left_childref, right_childref);
+  //     inout self.Insert(ref, node);
+  //   }
 
-    /// Temporary node borrow methods
+  //   /// Temporary node borrow methods
 
-    shared method GetNodeInfo(ref: BT.G.Reference)
-    returns (pivots: Pivots.PivotTable, children: Option<seq<BT.G.Reference>>)
-    requires Inv()
-    requires ptr(ref).Some?
-    ensures pivots == I()[ref].pivotTable
-    ensures children == I()[ref].children
-    {
-      shared var node := Get(ref);
-      children := node.children;
-      pivots := node.pivotTable;
-    }
+  //   shared method GetNodeInfo(ref: BT.G.Reference)
+  //   returns (pivots: Pivots.PivotTable, children: Option<seq<BT.G.Reference>>)
+  //   requires Inv()
+  //   requires ptr(ref).Some?
+  //   ensures pivots == I()[ref].pivotTable
+  //   ensures children == I()[ref].children
+  //   {
+  //     shared var node := Get(ref);
+  //     children := node.children;
+  //     pivots := node.pivotTable;
+  //   }
 
-    shared method GetNodeBucketsLen(ref: BT.G.Reference)
-    returns (len: uint64)
-    requires Inv()
-    requires ptr(ref).Some?
-    ensures len as nat == |I()[ref].buckets|
-    {
-      shared var node := Get(ref);
-      len := lseq_length_as_uint64(node.buckets);
-    }
+  //   shared method GetNodeBucketsLen(ref: BT.G.Reference)
+  //   returns (len: uint64)
+  //   requires Inv()
+  //   requires ptr(ref).Some?
+  //   ensures len as nat == |I()[ref].buckets|
+  //   {
+  //     shared var node := Get(ref);
+  //     len := lseq_length_as_uint64(node.buckets);
+  //   }
 
-    shared method GetMessage(ref: BT.G.Reference, i: uint64, key: KeyType.Key)
-    returns (msg: Option<Message>)
-    requires Inv()
-    requires ptr(ref).Some?
-    requires BT.WFNode(I()[ref])
-    requires Pivots.BoundedKey(I()[ref].pivotTable, key)
-    requires i as int == Pivots.Route(I()[ref].pivotTable, key)
-    ensures 
-      && var bucket := I()[ref].buckets[i];
-      && msg == BucketsLib.bucketBinarySearchLookup(bucket, key)
-    {
-      shared var node := Get(ref);
-      msg := lseq_peek(node.buckets, i).Query(key);
-    }
+  //   shared method GetMessage(ref: BT.G.Reference, i: uint64, key: KeyType.Key)
+  //   returns (msg: Option<Message>)
+  //   requires Inv()
+  //   requires ptr(ref).Some?
+  //   requires BT.WFNode(I()[ref])
+  //   requires Pivots.BoundedKey(I()[ref].pivotTable, key)
+  //   requires i as int == Pivots.Route(I()[ref].pivotTable, key)
+  //   ensures 
+  //     && var bucket := I()[ref].buckets[i];
+  //     && msg == BucketsLib.bucketBinarySearchLookup(bucket, key)
+  //   {
+  //     shared var node := Get(ref);
+  //     msg := lseq_peek(node.buckets, i).Query(key);
+  //   }
 
-    shared method NodeBucketsWeight(ref: BT.G.Reference)
-    returns (weight: uint64)
-    requires Inv()
-    requires ptr(ref).Some?
-    requires BT.WFNode(I()[ref])
-    ensures weight as int == WeightBucketList(I()[ref].buckets)
-    {
-      shared var node := Get(ref);
-      weight := MutBucket.computeWeightOfSeq(node.buckets);
-    }
+  //   shared method NodeBucketsWeight(ref: BT.G.Reference)
+  //   returns (weight: uint64)
+  //   requires Inv()
+  //   requires ptr(ref).Some?
+  //   requires BT.WFNode(I()[ref])
+  //   ensures weight as int == WeightBucketList(I()[ref].buckets)
+  //   {
+  //     shared var node := Get(ref);
+  //     weight := MutBucket.computeWeightOfSeq(node.buckets);
+  //   }
 
-    shared method NodeBoundedBucket(ref: BT.G.Reference, 
-      pivotsref: BT.G.Reference, slot: uint64)
-    returns (b: bool)
-    requires Inv()
-    requires ref in I()
-    requires pivotsref in I()
-    requires BT.WFNode(I()[ref])
-    requires BT.WFNode(I()[pivotsref])
-    requires slot as nat < |I()[ref].buckets|
-    ensures b == Pivots.BoundedKeySeq(I()[pivotsref].pivotTable,
-        I()[ref].buckets[slot as nat].keys)
-    {
-      shared var node := Get(ref);
-      if ref == pivotsref {
-        b := node.BoundedBucket(node.pivotTable, slot);
-      } else {
-        shared var pivotsnode := Get(pivotsref);
-        b := node.BoundedBucket(pivotsnode.pivotTable, slot);
-      }
-    }
+  //   shared method NodeBoundedBucket(ref: BT.G.Reference, 
+  //     pivotsref: BT.G.Reference, slot: uint64)
+  //   returns (b: bool)
+  //   requires Inv()
+  //   requires ref in I()
+  //   requires pivotsref in I()
+  //   requires BT.WFNode(I()[ref])
+  //   requires BT.WFNode(I()[pivotsref])
+  //   requires slot as nat < |I()[ref].buckets|
+  //   ensures b == Pivots.BoundedKeySeq(I()[pivotsref].pivotTable,
+  //       I()[ref].buckets[slot as nat].keys)
+  //   {
+  //     shared var node := Get(ref);
+  //     if ref == pivotsref {
+  //       b := node.BoundedBucket(node.pivotTable, slot);
+  //     } else {
+  //       shared var pivotsnode := Get(pivotsref);
+  //       b := node.BoundedBucket(pivotsnode.pivotTable, slot);
+  //     }
+  //   }
 
-    shared method NodePartialFlush(parentref: BT.G.Reference, 
-      childref: BT.G.Reference, slot: uint64)
-    returns (linear newparentBucket: MutBucket, linear newchild: Node)
-    requires Inv()
-    requires parentref in I()
-    requires childref in I()
-    requires BT.WFNode(I()[parentref])
-    requires BT.WFNode(I()[childref])
-    requires slot as nat < |I()[parentref].buckets|
-    ensures newparentBucket.Inv()
-    ensures newchild.Inv()
-    ensures newchild.I().pivotTable == I()[childref].pivotTable
-    ensures newchild.I().children == I()[childref].children
-    ensures BucketModel.partialFlushResult(newparentBucket.I(), newchild.I().buckets)
-        == BucketModel.partialFlush(I()[parentref].buckets[slot], 
-          I()[childref].pivotTable, I()[childref].buckets)
-    {
-      shared var parent := Get(parentref);
-      shared var child := Get(childref);
+  //   shared method NodePartialFlush(parentref: BT.G.Reference, 
+  //     childref: BT.G.Reference, slot: uint64)
+  //   returns (linear newparentBucket: MutBucket, linear newchild: Node)
+  //   requires Inv()
+  //   requires parentref in I()
+  //   requires childref in I()
+  //   requires BT.WFNode(I()[parentref])
+  //   requires BT.WFNode(I()[childref])
+  //   requires slot as nat < |I()[parentref].buckets|
+  //   ensures newparentBucket.Inv()
+  //   ensures newchild.Inv()
+  //   ensures newchild.I().pivotTable == I()[childref].pivotTable
+  //   ensures newchild.I().children == I()[childref].children
+  //   ensures BucketModel.partialFlushResult(newparentBucket.I(), newchild.I().buckets)
+  //       == BucketModel.partialFlush(I()[parentref].buckets[slot], 
+  //         I()[childref].pivotTable, I()[childref].buckets)
+  //   {
+  //     shared var parent := Get(parentref);
+  //     shared var child := Get(childref);
 
-      WeightBucketLeBucketList(parent.I().buckets, slot as int);
-      assert WeightBucketList(child.I().buckets) <= MaxTotalBucketWeight();
+  //     WeightBucketLeBucketList(parent.I().buckets, slot as int);
+  //     assert WeightBucketList(child.I().buckets) <= MaxTotalBucketWeight();
 
-      linear var newpbucket, newbuckets := BucketImpl.PartialFlush(
-        lseq_peek(parent.buckets, slot as uint64), child.buckets, child.pivotTable);
+  //     linear var newpbucket, newbuckets := BucketImpl.PartialFlush(
+  //       lseq_peek(parent.buckets, slot as uint64), child.buckets, child.pivotTable);
 
-      newchild := Node(child.pivotTable, child.children, newbuckets);
-      newparentBucket := newpbucket;
-    }
+  //     newchild := Node(child.pivotTable, child.children, newbuckets);
+  //     newparentBucket := newpbucket;
+  //   }
 
     shared method NodeSplitMiddle(ref: BT.G.Reference)
     returns (linear left: MutBucket, linear right: MutBucket, pivot: Key)
@@ -475,7 +480,6 @@ module CacheImpl {
     returns (linear g: BGI.Generator)
     requires Inv()
     requires ptr(ref).Some?
-    requires BT.WFNode(I()[ref])
     requires r as nat < |I()[ref].buckets|
     ensures g.Basic?
     ensures g.biter.bucket == I()[ref].buckets[r as nat]
@@ -526,375 +530,5 @@ module CacheImpl {
   {
     cache.LemmaSizeEqCount();
     cache.cache.count
-  }
-
-  // boxed cache
-  // TODO(Jialin): switch to boxedoption
-  class MutCache {
-    var box: BoxedLinear<LMutCache>;
-    ghost var Repr: set<object>;
-
-    function Read() : LMutCache
-    requires box.Inv()
-    reads this, box, box.Repr
-    {
-      box.Read()
-    }
-
-    protected predicate Inv()
-    reads this, Repr
-    ensures Inv() ==> this in Repr
-    {
-      && box in Repr
-      && Repr == {this} + box.Repr
-      && box.Inv()
-      && box.Has()
-      && Read().Inv()
-    }
-
-    constructor ()
-    ensures Inv()
-    ensures I() == map[]
-    ensures fresh(Repr)
-    {
-      linear var cache := LMutCache.NewCache();
-      box := new BoxedLinear(cache);
-      new;
-      Repr := {this} + box.Repr;
-    }
-    
-    method DebugAccumulate()
-    returns (acc: DebugAccumulator.DebugAccumulator)
-    requires box.Inv()
-    requires box.Has()
-    requires false
-    {
-     acc := LMutCache.DebugAccumulate(box.Borrow());
-    }
-
-    protected function I() : map<BT.G.Reference, BT.G.Node>
-    requires Inv()
-    reads Repr
-    {
-      Read().I()
-    }
-
-    protected function ptr(ref: BT.G.Reference) : Option<Node>
-    requires Inv()
-    reads this, box, box.Repr
-    ensures ptr(ref).None? ==> ref !in I()
-    ensures ptr(ref).Some? ==>
-        && ref in I()
-        && ptr(ref).value.Inv()
-        && I()[ref] == ptr(ref).value.I()
-    {
-      Read().ptr(ref)
-    }
-
-    method InCache(ref: BT.G.Reference) returns (b: bool)
-    requires Inv()
-    ensures b == ptr(ref).Some?
-    {
-      b := this.box.Borrow().InCache(ref);
-    }
-
-    method Insert(ref: BT.G.Reference, linear node: Node)
-    requires Inv()
-    requires node.Inv()
-    requires |I()| <= 0x10000
-    ensures Inv()
-    ensures I() == old(I()[ref := node.I()])
-    ensures forall r | r != ref :: ptr(r) == old(ptr(r))
-    ensures Repr == old(Repr)
-    modifies this.Repr
-    {
-      linear var c := this.box.Take();
-      inout c.Insert(ref, node);
-      this.box.Give(c);
-    }
-
-    method ReplaceAndGet(ref: BT.G.Reference, linear newNode: Node)
-    returns (linear oldNode: Node)
-    requires Inv()
-    requires newNode.Inv()
-    requires ptr(ref).Some?
-    requires |I()| <= 0x10000
-    ensures Inv()
-    ensures oldNode.Inv()
-    ensures |I()| == |old(I())|
-    ensures oldNode == old(ptr(ref)).value
-    ensures I() == old(I())[ref := newNode.I()]
-    ensures forall r | r != ref :: ptr(r) == old(ptr(r))
-    ensures Repr == old(Repr)
-    modifies this.Repr
-    {
-      linear var c := this.box.Take();
-      oldNode := inout c.ReplaceAndGet(ref, newNode);
-      this.box.Give(c);
-    }
-
-    method RemoveAndGet(ref: BT.G.Reference) returns (linear node: Node)
-    requires Inv()
-    requires ptr(ref).Some?
-    ensures Inv()
-    ensures node.Inv()
-    ensures node == old(ptr(ref)).value
-    ensures I() == MapRemove1(old(I()), ref)
-    ensures Repr == old(Repr)
-    modifies this.Repr
-    {
-      linear var c := this.box.Take();
-      node := inout c.RemoveAndGet(ref);
-      this.box.Give(c);
-    }
-
-    method Remove(ref: BT.G.Reference)
-    requires Inv()
-    ensures Inv()
-    ensures I() == MapRemove1(old(I()), ref)
-    ensures Repr == old(Repr)
-    modifies this.Repr
-    {
-      linear var c := this.box.Take();
-      inout c.Remove(ref);
-      this.box.Give(c);
-    }
-
-    // This is used for the 'grow' operation.
-    method MoveAndReplace(oldref: BT.G.Reference,
-      newref: BT.G.Reference, linear node: Node)
-    requires Inv()
-    requires node.Inv()
-    requires |I()| <= 0x10000
-    requires oldref in I()
-    ensures Inv()
-    ensures I() == old(I())[oldref := node.I()][newref := old(I())[oldref]]
-    ensures Repr == old(Repr)
-    modifies this.Repr
-    {
-      linear var c := this.box.Take();
-      inout c.MoveAndReplace(oldref, newref, node);
-      this.box.Give(c);
-    }
-
-    // Like Insert, but with slightly different requires
-    method Overwrite(ref: BT.G.Reference, linear node: Node)
-    requires Inv()
-    requires node.Inv()
-    requires ref in I()
-    requires |I()| <= 0x10000
-    ensures Inv()
-    ensures I() == old(I())[ref := node.I()]
-    ensures Repr == old(Repr)
-    modifies this.Repr
-    {
-      linear var c := this.box.Take();
-      inout c.Overwrite(ref, node);
-      this.box.Give(c);
-    }
-
-    function method Count() : (c : uint64)
-    requires Inv()
-    reads this, Repr
-    ensures c as int == |I()|
-    {
-      CacheCount(this.box.Borrow())
-    }
-
-    method NodeUpdateSlot(ref: BT.G.Reference, slot: uint64, 
-      linear bucket: MutBucket, childref: BT.G.Reference)
-    returns (newchildren: Option<seq<BT.G.Reference>>)
-    requires Inv()
-    requires bucket.Inv()
-    requires ptr(ref).Some?
-    requires BT.WFNode(I()[ref])
-    requires |I()| <= 0x10000
-    requires I()[ref].children.Some?
-    requires slot as nat < |I()[ref].children.value|
-    requires slot as int + 1 < 0x1_0000_0000_0000_0000
-    ensures Inv()
-    ensures I() == old(I()[ref := BT.G.Node(
-        I()[ref].pivotTable,
-        Some(I()[ref].children.value[slot as int := childref]),
-        I()[ref].buckets[slot as int := bucket.bucket]
-      )])
-    ensures newchildren == I()[ref].children
-    ensures Repr == old(Repr)
-    modifies this.Repr
-    {
-      linear var c := this.box.Take();
-      newchildren := inout c.NodeUpdateSlot(ref, slot, bucket, childref);
-      this.box.Give(c);
-    }
-
-    method InsertKeyValue(ref: BT.G.Reference, key: Key, msg: Message)
-    requires Inv()
-    requires ref in I()
-    requires ptr(ref).Some?
-    requires |I()| <= 0x10000
-    requires BT.WFNode(I()[ref])
-    requires Pivots.BoundedKey(I()[ref].pivotTable, key)
-    requires WeightBucketList(I()[ref].buckets) + WeightKey(key) 
-      + WeightMessage(msg) < 0x1_0000_0000_0000_0000
-    ensures Inv()
-    ensures I() == old(I()[ref := BT.NodeInsertKeyValue(I()[ref], key, msg)])
-    ensures Repr == old(Repr)
-    modifies this.Repr
-    {
-      linear var c := this.box.Take();
-      inout c.InsertKeyValue(ref, key, msg);
-      this.box.Give(c);
-    }
-
-    method SplitParent(ref: BT.G.Reference, slot: uint64, pivot: Key,
-      left_childref: BT.G.Reference, right_childref: BT.G.Reference)
-    requires Inv()
-    requires ptr(ref).Some?
-    requires BT.WFNode(I()[ref])
-    requires I()[ref].children.Some?
-    requires 0 <= slot as int < |I()[ref].children.value|
-    requires 0 <= slot as int < |I()[ref].buckets|
-    requires |I()| <= 0x10000
-    ensures Inv()
-    ensures I() == old(I()[ref := BT.SplitParent(I()[ref],
-      pivot, slot as int, left_childref, right_childref)])
-    ensures Repr == old(Repr)
-    modifies this.Repr
-    {
-      linear var c := this.box.Take();
-      inout c.SplitParent(ref, slot, pivot, left_childref, right_childref);
-      this.box.Give(c);
-    }
-
-    /// temporary node methods
-    method GetNodeInfo(ref: BT.G.Reference)
-    returns (pivots: Pivots.PivotTable, children: Option<seq<BT.G.Reference>>)
-    requires Inv()
-    requires ptr(ref).Some?
-    ensures pivots == I()[ref].pivotTable
-    ensures children == I()[ref].children
-    {
-      pivots, children := this.box.Borrow().GetNodeInfo(ref);
-    }
-
-    method GetNodeBucketsLen(ref: BT.G.Reference)
-    returns (len: uint64)
-    requires Inv()
-    requires ptr(ref).Some?
-    ensures len as nat == |I()[ref].buckets|
-    {
-      len := this.box.Borrow().GetNodeBucketsLen(ref);
-    }
-
-    method GetMessage(ref: BT.G.Reference, i: uint64, key: KeyType.Key)
-    returns (msg: Option<Message>)
-    requires Inv()
-    requires ptr(ref).Some?
-    requires BT.WFNode(I()[ref])
-    requires Pivots.BoundedKey(I()[ref].pivotTable, key)
-    requires i as int == Pivots.Route(I()[ref].pivotTable, key)
-    ensures 
-      && var bucket := I()[ref].buckets[i];
-      && msg == BucketsLib.bucketBinarySearchLookup(bucket, key)
-    {
-      msg := this.box.Borrow().GetMessage(ref, i, key);
-    }
-
-    method NodeBucketsWeight(ref: BT.G.Reference) returns (weight: uint64)
-    requires Inv()
-    requires ptr(ref).Some?
-    requires BT.WFNode(I()[ref])
-    ensures weight as int == WeightBucketList(I()[ref].buckets)
-    {
-      weight := this.box.Borrow().NodeBucketsWeight(ref);
-    }
-  
-    method NodeBoundedBucket(ref: BT.G.Reference, 
-      pivotsref: BT.G.Reference, slot: uint64) returns (b: bool)
-    requires Inv()
-    requires ref in I()
-    requires pivotsref in I()
-    requires BT.WFNode(I()[ref])
-    requires BT.WFNode(I()[pivotsref])
-    requires slot as nat < |I()[ref].buckets|
-    ensures b == Pivots.BoundedKeySeq(I()[pivotsref].pivotTable,
-        I()[ref].buckets[slot as nat].keys)
-    {
-      b := this.box.Borrow().NodeBoundedBucket(ref, pivotsref, slot);
-    }
-
-    method NodePartialFlush(parentref: BT.G.Reference, 
-      childref: BT.G.Reference, slot: uint64)
-    returns (linear newparentBucket: MutBucket, linear newchild: Node)
-    requires Inv()
-    requires parentref in I()
-    requires childref in I()
-    requires BT.WFNode(I()[parentref])
-    requires BT.WFNode(I()[childref])
-    requires slot as nat < |I()[parentref].buckets|
-    ensures newparentBucket.Inv()
-    ensures newchild.Inv()
-    ensures newchild.I().pivotTable == I()[childref].pivotTable
-    ensures newchild.I().children == I()[childref].children
-    ensures BucketModel.partialFlushResult(newparentBucket.I(), newchild.I().buckets)
-        == BucketModel.partialFlush(I()[parentref].buckets[slot],
-          I()[childref].pivotTable, I()[childref].buckets)
-    {
-      newparentBucket, newchild := this.box.Borrow().NodePartialFlush(parentref, childref, slot);
-    }
-
-    method NodeSplitMiddle(ref: BT.G.Reference)
-    returns (linear left: MutBucket, linear right: MutBucket, pivot: Key)
-    requires Inv()
-    requires ref in I()
-    requires BT.WFNode(I()[ref])
-    requires |I()[ref].buckets| == 1
-    ensures left.Inv()
-    ensures right.Inv()
-    ensures
-      && var bucket := I()[ref].buckets[0];
-      && pivot == BucketsLib.getMiddleKey(bucket)
-      && left.I() == BucketsLib.SplitBucketLeft(bucket, pivot)
-      && right.I() == BucketsLib.SplitBucketRight(bucket, pivot)
-    {
-      left, right, pivot := this.box.Borrow().NodeSplitMiddle(ref);
-    }
-
-    method NodeCutOff(ref: BT.G.Reference, lbound: KeyType.Key,ubound: Option<KeyType.Key>)
-    returns (linear node': Node)
-    requires Inv()
-    requires ptr(ref).Some?
-    requires BT.WFNode(I()[ref])
-    requires BT.ValidSplitKey(I()[ref], lbound, ubound)
-    ensures node'.Inv()
-    ensures node'.I() == BT.CutoffNode(I()[ref], lbound, ubound)
-    {
-      node' := this.box.Borrow().NodeCutOff(ref, lbound, ubound);
-    }
-
-    method NodeBucketGen(ref: BT.G.Reference, r: uint64, start: BT.UI.RangeStart)
-    returns (linear g: BGI.Generator)
-    requires Inv()
-    requires ptr(ref).Some?
-    requires BT.WFNode(I()[ref])
-    requires r as nat < |I()[ref].buckets|
-    ensures g.Basic?
-    ensures g.biter.bucket == I()[ref].buckets[r as nat]
-    ensures g.Inv()
-    ensures g.I() == BGI.BucketGeneratorModel.GenFromBucketWithLowerBound(
-        I()[ref].buckets[r as nat], start)
-    {
-      g := this.box.Borrow().NodeBucketGen(ref, r, start);
-    }
-
-    method NodeBiggestSlot(ref: BT.G.Reference)
-    returns (res : (uint64, uint64))
-    requires Inv()
-    requires ptr(ref).Some?
-    requires FPM.biggestSlot.requires(I()[ref].buckets)
-    ensures res == FPM.biggestSlot(I()[ref].buckets)
-    {
-      res := this.box.Borrow().NodeBiggestSlot(ref);
-    }
   }
 }
